Risc0/Basic.lean
@@ -220,6 +220,44 @@ lemma valid_init' : (init m n input output hIn hOut).WellFormed where
 
 lemma valid_init : (init_default m n).WellFormed := valid_init'
 
+lemma l {a b} {m: List α} (h_a : a ∈ m) (h_b : ¬b ∈ m) : a ≠ b := by
+  aesop
+lemma addBuffer_preserves_wellformed {st: State} {name: String} {buffer: Buffer}
+  (h_wf: st.WellFormed) (h_distinct: ¬⟨name⟩ ∈ st.vars) (h_cycle: buffer.length = st.cycle + 1):
+  (st.addBuffer name buffer).WellFormed where
+  distinct := by
+    unfold addBuffer 
+    simp [h_distinct, h_wf.distinct]
+  hVars := by
+    unfold varsConsistent addBuffer
+    aesop
+    . show var ∈ st.buffers[⟨name⟩] := buffer -- with var ∈ vars
+      have var_not_name: var ≠ ⟨name⟩ := l (m := st.vars) h h_distinct
+      have var_in_buffers: var ∈ st.buffers := Iff.mp (h_wf.hVars var) h
+      exact Map.mem_skip var_in_buffers
+    . show var = { name := name } ∨ var ∈ st.vars -- with var ∈ st.buffers[⟨name⟩] := buffer
+      have h': var = { name := name } ∨ var ∈ st.buffers := Map.mem_unroll_assignment.mp a
+      cases h' with
+      | inl hp => apply Or.inl; exact hp
+      | inr hq => apply Or.inr; exact (h_wf.hVars var).mpr hq
+  hCycle := by {
+    unfold cycleIsRows
+    intros var h_var
+    simp [h_var]
+    unfold Map.get addBuffer
+    simp [Map.update]
+    aesop
+    have h_var_in_buffers: var ∈ st.buffers := by {
+      unfold addBuffer at h_var
+      simp [Map.mem_skip] at h_var
+      sorry -- WIP stopped here
+    }
+    sorry
+  }
+  hCols := sorry
+  hColsLen := sorry
+
+
 def update (state : State) (name : String) (x : Option Lit) : State :=
   match x with
     | .none => {state with isFailed := true}
